Examples.lean
@@ -1,1 +1,2 @@
-import Examples.Truth
+import Examples.Pow.Correct
+import Examples.Truth.Correct
